compiler/src/ProgramSpec.v
@@ -26,7 +26,7 @@ Section Params1.
        but might not hold in the middle of the loop because more needs to be appended *)
     goodTrace: Semantics.trace -> Prop;
     (* state invariant which holds at the beginning (and end) of each loop iteration *)
-    isReady: Semantics.trace -> Semantics.mem -> Semantics.locals -> MetricLog -> Prop;
+    isReady: Semantics.trace -> Semantics.mem -> Semantics.locals -> Prop;
   }.
 
   Definition mem_available(start pastend: Semantics.word)(m: Semantics.mem): Prop :=
@@ -45,13 +45,13 @@ Section Params1.
     init_code_correct: forall m0 l0 mc0,
       mem_available spec.(datamem_start) spec.(datamem_pastend) m0 ->
       exec prog.(funimpls) prog.(init_code) nil m0 l0 mc0
-        (fun t' m' l' mc' => spec.(isReady) t' m' l' mc' /\ spec.(goodTrace) t');
+        (fun t' m' l' mc' => spec.(isReady) t' m' l' /\ spec.(goodTrace) t');
 
     loop_body_correct: forall t m l mc,
-       spec.(isReady) t m l mc ->
+       spec.(isReady) t m l ->
        spec.(goodTrace) t ->
        exec prog.(funimpls) prog.(loop_body) t m l mc
-        (fun t' m' l' mc' => spec.(isReady) t' m' l' mc' /\ spec.(goodTrace) t');
+        (fun t' m' l' mc' => spec.(isReady) t' m' l' /\ spec.(goodTrace) t');
   }.
 
 End Params1.
